Sync

Unify.v
@@ -1,96 +1,161 @@
-Require Export List.
+Require Import List.
 Import ListNotations.
-Require Export Arith.
-Require Export Omega.
-Require Export FMapAVL.
-Require Export Coq.Structures.OrderedTypeEx.
+Require Import Arith.
+Require Import Omega.
 
-Inductive Term : Type :=
-| V : nat -> Term
-| C : nat -> list Term -> Term.
+(************************* Terms *************************)
+(* Name of entities *)
+Definition name := nat.
 
-Module S := FMapAVL.Make (Nat_as_OT).
+(* Term type *) 
+Inductive term : Set :=
+(* a variable           *) | Var : name -> term
+(* a constant           *) | Cst : name -> term
+(* a binary constructor *) | Con : name -> term -> term -> term.
 
-Definition Subst: Type := S.t Term.
-
-Definition empty : Subst := S.empty Term.
-
-Definition find k (m: Subst) := S.find k m.
-
-Definition update (k: nat) (v: Term) (m: Subst) :=
-  S.add k v m.
-
-Notation "s [ k <- v ]" := (update k v s) (at level 0).
-Reserved Notation "t \ s" (at level 0).
-
-Fixpoint apply (s: Subst) (t: Term) : Term := 
+(* Occurs property *)
+Fixpoint occurs (n : name) (t : term) : bool :=
   match t with
-  | V v    => match find v s with
-              | None   => V v
-              | Some t => t
-              end
-  | C c ts => C c (map (fun t => t \ s) ts)
-  end
-where "t \ s" := (apply s t).
-
-(*
--- Unification
-unify :: Maybe Sigma -> Ts -> Ts -> Maybe Sigma 
-unify Nothing _ _ = Nothing
-unify st@(Just subst) u v = 
-  unify' (walk u subst) (walk v subst)  where
-    unify' (V u) (V v) | u == v = Just subst
-    unify' (V u) _              = Just $ (u, v) : subst
-    unify' _ (V v)              = Just $ (v, u) : subst
-    unify' (C a as) (C b bs) | a == b && length as == length bs = 
-      foldl (\ st (u, v) -> unify st u v) st $ zip as bs
-    unify' _ _ = Nothing
-    walk x@(V v) s =
-      case lookup v s of
-        Nothing -> x
-        Just t  -> walk t s
-    walk u     _ = u
-*)
-
-Print well_founded.
-Print Acc.
-Check Fix.
-
-Definition sizeOrder (s1 s2 : Subst) := S.cardinal s1 < S.cardinal s2.
-
-Hint Constructors Acc.
-
-Lemma sizeOrder_wf': forall (size: nat) (s: Subst), S.cardinal s < size -> Acc sizeOrder s.
-  unfold sizeOrder. induction size.  
-    intros. inversion H.
-    intros. constructor. intros. apply IHsize. omega.
-Defined.
- 
-Theorem sizeOrder_wf: well_founded sizeOrder.
-  red; intro; eapply sizeOrder_wf'; eauto.
-Defined.
-
-Lemma remove_wf: forall (s: Subst) (n: nat) (t: Term),
-  find n s = Some t -> sizeOrder (S.remove n s) s.
-  intros. red. 
-
-
-Fixpoint walk (t: Term) (s: Subst) : Term :=
-  match t with
-  | V n => match find n s with
-           | None   => V n
-           | Some t => walk t (S.remove n s)
-           end
-  | t => t
+  | Var n1    => if eq_nat_dec n1 n then true else false
+  | Con _ l r => orb (occurs n l) (occurs n r)
+  | _         => false
   end.
+
+(******************** Substitutions **********************)
+(* Substitution *)
+Definition subst : Type := list (name * term).
+
+(* Substitution domain *)
+Fixpoint domain (s : subst) : list name := map (@fst name term) s.
   
+(* Substitution image *)
+Fixpoint image (s : subst) (n : name) : option term :=
+  match s with
+  | [] => None
+  | (m, t) :: tl => if eq_nat_dec m n then Some t else image tl n
+  end.
 
+(* Substitution application *)
+Fixpoint apply (s : subst) (t : term) : term :=
+  match t with
+  | Cst _     => t
+  | Var n     => match image s n with None => t | Some t' => t' end
+  | Con n l r => Con n (apply s l) (apply s r)
+  end.
 
-Example ex1: find 3 (empty [1 <- V 2][3 <- V 4]) = Some (V 4).
-Proof. reflexivity. Qed.
+(* Generality *)
+Definition more_general (m s : subst) : Prop :=
+  exists (s' : subst), forall (t : term), apply s t = apply s' (apply m t).
 
-Example ex2: find 5 (empty [1 <- V 2][3 <- V 4]) = None.
-Proof. reflexivity. Qed.
+(* Unification property *)
+Definition unifier (s : subst) (t1 t2 : term) : Prop := apply s t1 = apply s t2.
 
+(* MGU *)
+Definition mgu (m : subst) (t1 t2 : term) : Prop :=
+  unifier m t1 t2 /\ forall (s : subst), unifier s t1 t2 -> more_general m s.
 
+(******************** Well-formed Substitutions ***********)
+(* Substitution welformedness *)
+Definition subst_wf (s : subst) : Prop :=
+  forall (m n : name), forall (t : term), In m (domain s) -> image s n = Some t -> occurs m t = false.
 
+(* Well-formed substitution *)
+Definition swbst := {s : subst | subst_wf s}.
+
+(* Coercion *)
+Definition coerce (T : Type) (P : subst -> T) (s: swbst) : T :=
+  match s with exist l _ => P l end.
+             
+(* Empty well-formed substitution *)
+Definition empty : subst := [].
+(*
+Proof.
+  exists []. unfold subst_wf. intros. simpl in H. inversion H.
+Qed.
+*)
+(* Extending a well-fromed substitution *)
+Definition extend (b : subst) (n : name) (t : term) := (n, apply b t) :: b.
+
+(* Singleton substitution *)
+Definition trivial (n : name) (t : term) : subst := extend empty n t.
+(*
+(* Singleton well-formed substitution construction *)
+Definition trivial (n : name) (t : term) : option swbst.
+Proof.
+  remember (occurs n t). destruct b.
+  * exact None.
+  * remember [(n, t)]. assert (A: image l n = Some t). rewrite Heql. simpl.
+    destruct (eq_nat_dec n n). auto. exfalso. auto. refine (Some _). exists l.
+    rewrite Heql. unfold subst_wf. intros. simpl in H.
+    destruct (eq_nat_dec n n0). inversion H. subst. auto. inversion H.
+Qed.
+ *)
+
+Inductive outcome : Set :=
+| Fail
+| Fine
+| Subst : forall (n: name) (t: term), outcome.  
+
+Definition create (n: name) (t: term) : outcome :=
+  if occurs n t then Fail else Subst n t.
+(*.
+  remember (occurs n t). destruct b.
+  * exact Fail.
+  * symmetry in Heqb. exact (Subst n t Heqb).
+Defined.
+  *)         
+(* Find a difference in a couple of terms and try to make a unification step *)
+Fixpoint delta (t1 t2 : term) : outcome :=
+  match (t1, t2) with
+  | (Cst n1      , Cst n2      ) => if eq_nat_dec n1 n2 then Fine else Fail 
+  | (Con n1 l1 r1, Con n2 l2 r2) => if eq_nat_dec n1 n2
+                                    then
+                                      match delta l1 l2 with
+                                      | Fail => Fail
+                                      | Fine => delta r1 r2
+                                      | res  => res
+                                      end
+                                    else Fail
+  | (Var n1      , Var n2      ) => if eq_nat_dec n1 n2 then Fine else create n1 t2
+  | (Var n1      , _           ) => create n1 t2
+  | (_           , Var n2      ) => create n2 t1
+  | (_           , _           ) => Fail
+  end.
+
+(* A distance between terms *)
+Fixpoint distance (t1 t2 : term) : nat :=
+  match (t1, t2) with
+  | (Cst n1      , Cst n2      ) => if eq_nat_dec n1 n2 then 0 else 1 
+  | (Con n1 l1 r1, Con n2 l2 r2) => if eq_nat_dec n1 n2
+                                    then distance l1 l2 + distance r1 r2
+                                    else 1
+  | (Var n1      , Var n2      ) => if eq_nat_dec n1 n2 then 0 else 1
+  | (_           , _           ) => 1
+  end.
+
+Lemma apply_eq: forall (t1 t2 : term) (n : name), occurs n t1 = false -> apply [(n, t2)] t1 = t1.
+Proof. admit. Admitted.
+
+Lemma apply_empty: forall (t1 : term), apply [] t1 = t1.
+Proof. admit. Admitted.
+
+Lemma distance_eq_zero: forall (t : term), distance t t = 0.
+Proof. admit. Admitted.
+                       
+Lemma distance_decrease:
+  forall (t1 t2 t: term) (n: name),
+    delta t1 t2 = Subst n t -> distance t1 t2 > distance (apply (trivial n t) t1) (apply (trivial n t) t2).
+Proof.
+  intros. induction t1.
+  * unfold delta in H. unfold create in H. destruct t2. destruct (eq_nat_dec n0 n1). inversion H.
+    destruct (occurs n0 (Var n1)). inversion H. inversion H. subst. unfold trivial. unfold empty. unfold extend. unfold apply.
+    simpl. destruct (eq_nat_dec n n1). rewrite e in n2. exfalso. auto. destruct (eq_nat_dec n n). unfold distance.
+    destruct (eq_nat_dec n1 n1). omega. exfalso. auto. exfalso. auto.
+    unfold occurs in H. inversion H.  unfold trivial. unfold empty. unfold extend. unfold apply.
+    simpl. destruct (eq_nat_dec n n). simpl. destruct (eq_nat_dec n1 n1). omega. exfalso. auto. exfalso. auto.
+    destruct (occurs n0 (Con n1 t2_1 t2_2)) eqn:D. inversion H. inversion H. unfold trivial. unfold empty. unfold extend.
+    apply apply_eq with (t2:=apply [] (Con n1 t2_1 t2_2)) in D. subst n0. rewrite D. rewrite apply_empty.
+    unfold apply. unfold image. destruct (eq_nat_dec n n). rewrite distance_eq_zero. unfold distance. omega. exfalso. auto.
+  * admit.
+  * 
+    
